Full proof working

compiler.v
@@ -5,6 +5,12 @@ From LF Require Import imports.
 From LF Require Import transforms.
 From LF Require Import python.
 
+Fixpoint convertValues (v : AbValue) : PyValue :=
+  match v with
+  | AbNat n => PyNat n
+  | AbBool b => PyBool b
+  end.
+
 Fixpoint numCompile (ae : AbNum) : PyNum :=
   match ae with
     | AbLit l => PyLit l
@@ -19,9 +25,22 @@ Fixpoint numExprCompile (ae : AbNumExpr) : PyNumExpr :=
     | AbMulti a1 a2 => PyMulti (numExprCompile a1) (numExprCompile a2)
   end.
 
+Fixpoint binExprCompile (b : AbBinExpr) : PyBinExpr :=
+  match b with
+  | BinTrue => PyBinTrue
+  | BinFalse => PyBinFalse
+  | AbUnaryOp b => PyUnaryOp (binExprCompile b)
+  | AbLe a1 a2 => PyLe (numExprCompile a1) (numExprCompile a2)
+  | AbEq a1 a2 => PyEq (numExprCompile a1) (numExprCompile a2)
+  | AbNotEq a1 a2 => PyNotEq (numExprCompile a1) (numExprCompile a2)
+  | AbAnd b1 b2 => PyAnd (binExprCompile b1) (binExprCompile b2)
+  | AbOr b1 b2 => PyOr (binExprCompile b1) (binExprCompile b2)
+  end.
+
 Fixpoint exprCompile (e : AbExpr) : PyExpr :=
   match e with
-    | Ab_Num_Expr n => Py_Num_Expr (numExprCompile n)
+  | Ab_Num_Expr n => Py_Num_Expr (numExprCompile n)
+  | Ab_Bin_Expr b => Py_Bin_Expr (binExprCompile b)
   end.
 
 Fixpoint compile (ac : AbCommand) : PyCommand :=
@@ -49,10 +68,27 @@ Proof.
     induction n; reflexivity.
 Qed.
 
-Theorem exprEquiv : forall ab st,
-    AbEval st ab = PyEval st (exprCompile ab).
+Theorem binExprEquiv : forall ab st,
+    AbEvalBin st ab = PyEvalBin st (binExprCompile ab).
 Proof.
-  intros. induction ab. apply numExprEquiv.
+  intros.
+  induction ab; simpl in *; try rewrite IHab; try reflexivity.
+  - (* AbLe -> PyLe *)
+    rewrite numExprEquiv. rewrite numExprEquiv. reflexivity.
+  - (* AbEq -> PyEq *)
+    rewrite numExprEquiv. rewrite numExprEquiv. reflexivity.
+  - (* AbNotEq -> PyNotEq *)
+    rewrite numExprEquiv. rewrite numExprEquiv. reflexivity.
+  - (* AbAnd -> PyAnd *)
+    rewrite IHab1. rewrite IHab2. reflexivity.
+  - (* AbOr -> PyOr *)
+    rewrite IHab1. rewrite IHab2. reflexivity.
+Qed.
+
+Theorem exprEquiv : forall ab st,
+    convertValues (AbEval st ab) = PyEval st (exprCompile ab).
+Proof.
+  intros. induction ab; simpl in *; try rewrite numExprEquiv; try rewrite binExprEquiv; reflexivity.
 Qed.
 
 Theorem compiler_correctness : forall a st st1 st2,
@@ -63,23 +99,24 @@ Proof.
   induction a.
   - (* AbTransform -> PyAssign *)
     induction a.
-    (* Ab_Num_Expr -> Py_Num_Expr *)
-    induction a; intros.
-    (* AbNum2 -> PyNum2 *)
+    + (* Ab_Num_Expr -> Py_Num_Expr *)
+      induction a; intros.
+      (* AbNum2 -> PyNum2 *)
       induction n; simpl in *; inversion H; inversion H0; subst; reflexivity.
-    + (* AbAdd -> PyAdd *)
-      inversion H.
-    + (* AbSub -> PySub *)
-      inversion H.
-    + (* AbMulti -> PyMulti *)
-      inversion H.
+      * (* AbAdd -> PyAdd *)
+        inversion H.
+      * (* AbSub -> PySub *)
+        inversion H.
+      * (* AbMulti -> PyMulti *)
+        inversion H.
+    + (* Ab_Bin_Expr -> Py_Bin_Expr *)
+      induction b; intros; inversion H.
   - (* AbSeq -> PySeq *)
-    intros st st1 st2 H1 H2.
-    
-    inversion H. inversion H0. subst.
-    induction a1; induction a2.
-    simpl in *.
-    
-    + (* AbTransform -> PyAssign *)
-      
+    intros st st'1 st'2 H1 H2.
+    inversion H1. inversion H2.
+    subst.
+    rewrite IHa2 with (st := st') (st1 := st'1) (st2 := st'2).
+    reflexivity.
+    assumption.
+    rewrite IHa1 with (st := st) (st1 := st') (st2 := st'0); assumption.  
 Qed.
