imports.v
@@ -6,7 +6,6 @@ Require Import Coq.Arith.Arith.
 Require Import Coq.Arith.EqNat.
 Require Import Coq.Lists.List.
 Require Export Coq.Strings.String.
-Require Export Coq.FSets.FMapList.
 Import ListNotations.
 
 From LF Require Export Maps.
@@ -15,3 +14,13 @@ Definition state := total_map nat.
 
 Reserved Notation "c1 '/' st '\\' st'"
                   (at level 40, st at level 39).
+
+Fixpoint leb (n m : nat) : bool :=
+  match n with
+  | O => true
+  | S n' =>
+      match m with
+      | O => false
+      | S m' => leb n' m'
+      end
+  end.
